Refactor, Cleanup
Renamed some variables, changed some implicit arguments, added helper
functions and some lemmas, created notation modules.

Structure.v
@@ -1,84 +1,79 @@
 Require Import Base Signature Term.
 
 Section structure.
-  Variable Σ : signature.
+  Context {Σ : signature}.
 
   Structure structure := {
       domain : Type;
-      interpF : forall f : FuncS Σ, vec domain (FuncArr f) -> domain;
-      interpP : forall P : PredS Σ, vec domain (PredArr P) -> Prop;
-      interpIP : forall P : IndPredS Σ, vec domain (IndPredArr P) -> Prop;
+      interpF : forall f : FuncS Σ, vec domain (fun_ar f) -> domain;
+      interpP : forall P : PredS Σ, vec domain (pred_ar P) -> Prop;
+      interpIP : forall P : IndPredS Σ, vec domain (indpred_ar P) -> Prop;
     }.
 End structure.
 
-Arguments domain {Σ}.
-Arguments interpF {Σ}.
-Arguments interpP {Σ}.
-Arguments interpIP {Σ}.
+Arguments structure : clear implicits.
+Arguments interpF {Σ M} _ _ : rename.
+Arguments interpP {Σ M} _ _ : rename.
+Arguments interpIP {Σ M} _ _ : rename.
 Notation "| M |" := (domain M) (no associativity, at level 150).
 
 Section environment.
-  Variable Σ : signature.
-  Variable M : structure Σ.
+  Context {Σ : signature} {M : structure Σ}.
 
-  Definition env_var := var -> |M|.
+  Definition env := var -> |M|.
 
-  Definition env_var_subst (ρ : env_var) (x : var) (d : |M|)
-    : var -> |M| :=
+  Definition env_subst (ρ : env) (x : var) (d : |M|) : var -> |M| :=
     fun (y : var) => if y =? x then d else ρ y.
 
-  Section extended_environment.
-    Variable ρvar : env_var.
-              
-    Fixpoint env (t : term Σ) : |M| :=
-      match t with
-      | TVar x => ρvar x
-      | TFunc f args => interpF M f (V.map env args)
-      end.
+  Fixpoint eval (ρ : env) (t : term Σ) : |M| :=
+    match t with
+    | TVar x => ρ x
+    | TFunc f args => interpF f (V.map (eval ρ) args)
+    end.
 
-    Definition env_vec n (v : vec (term Σ) n) : vec (|M|) n :=
-      V.map env v.
+  Definition eval_vec (ρ : env) {n} (v : vec (term Σ) n) : vec (|M|) n :=
+    V.map (eval ρ) v.
 
-    Fixpoint env_subst (t : term Σ) (x : var) (d : |M|) : |M| :=
-      match t with
-      | TVar y => env_var_subst ρvar x d y
-      | TFunc f args => interpF M f (V.map (fun st => env_subst st x d) args)
-      end.
-  End extended_environment.
-
-  Section lemma_2_1_5.
-    Variable ρvar : env_var.
-    Definition ρ := env ρvar.
-    Variable t : term Σ.
-    Variable x : var.
-
-    Lemma env_subst_sanity1 : forall (d : |M|),
-        ~ E.In (Var t) x -> env_subst ρvar t x d = env ρvar t.
-    Proof.
-      induction t as [v | f args IH] using term_better_ind;
-        intros d x_not_in_t.
-      - simpl; unfold env_var_subst; destruct (v =? x) eqn:eq_vx.
-        + exfalso. apply x_not_in_t. rewrite Nat.eqb_eq in eq_vx; subst.
-          constructor.
-        + reflexivity.
-      - simpl. f_equal. apply V.map_ext_in.
-        intros st Hin. rewrite V.Forall_forall in IH.
-        apply IH.
-        + assumption.
-        + intros x_in_var_st. apply x_not_in_t.
-          constructor. apply Exists_exists; exists st; intuition.
-    Qed. 
-
-    Lemma env_subst_sanity2 : forall (u : term Σ),
-        env_subst ρvar t x (ρ u) = ρ (term_var_subst t u x).
-    Proof.
-      intros u. induction t as [v | f args IH] using term_better_ind2.
-      - cbn. unfold env_var_subst. destruct (v =? x) eqn:E;
-          reflexivity.
-      - simpl. f_equal. rewrite V.map_map.
-        apply V.map_ext_in. intros st Hst.
-        apply IH. assumption.
-    Qed.
-      
-  End lemma_2_1_5.
+  Fixpoint eval_subst (ρ : env) (t : term Σ) (x : var) (d : |M|) : |M| :=
+    match t with
+    | TVar y => env_subst ρ x d y
+    | TFunc f args => interpF f (V.map (fun st => eval_subst ρ st x d) args)
+    end.
 End environment.
+
+Arguments env {Σ} M.
+
+Section lemma_2_1_5.
+  Context {Σ : signature} {M : structure Σ}.
+  Variable ρ : env M.
+  Variable t : term Σ.
+  Variable x : var.
+
+  Lemma eval_subst_sanity1 : forall (d : |M|),
+      ~ Var t x -> eval_subst ρ t x d = eval ρ t.
+  Proof.
+    induction t as [v | f args IH] using term_ind1;
+      intros d x_not_in_t.
+    - simpl; unfold env_subst; destruct (v =? x) eqn:eq_vx.
+      + exfalso. apply x_not_in_t. rewrite Nat.eqb_eq in eq_vx; subst.
+        constructor.
+      + reflexivity.
+    - simpl. f_equal. apply V.map_ext_in.
+      intros st Hin. rewrite V.Forall_forall in IH.
+      apply IH.
+      + assumption.
+      + intros x_in_var_st. apply x_not_in_t.
+        constructor. apply Exists_exists; exists st; intuition.
+  Qed.
+
+  Lemma eval_subst_sanity2 : forall (u : term Σ),
+      eval_subst ρ t x (eval ρ u) = eval ρ (term_var_subst t x u).
+  Proof.
+    intros u. induction t as [v | f args IH] using term_ind2.
+    - cbn. unfold env_subst. destruct (v =? x) eqn:E;
+        reflexivity.
+    - simpl. f_equal. rewrite V.map_map.
+      apply V.map_ext_in. intros st Hst.
+      apply IH. assumption.
+  Qed.
+End lemma_2_1_5.
