Term.v
@@ -1,84 +1,98 @@
 Require Import Base.
 Require Import Signature.
 
-Section term.
-  Variable Σ : signature.
-  Definition var := nat.
+Notation var := nat.
 
+Section term.
+  Context {Σ : signature}.
+
+  Unset Elimination Schemes.
+  
   (* Definition 2.1.2 *)
   Inductive term : Type :=
   | TVar : var -> term
   (* constant symbols are function symbols with arity 0 *)
-  | TFunc : forall f : FuncS Σ, vec term (FuncArr f) -> term.
+  | TFunc : forall f : FuncS Σ, vec term (fun_ar f) -> term.
 
-  Section term_better_ind.
-    Variable P : term -> Prop.
-    
-    Hypothesis Pbase : forall v, P (TVar v).
-    Hypothesis Pind : forall (f : FuncS Σ) (args : vec term (FuncArr f)),
-        V.Forall (fun st => P st) args -> P (TFunc f args).
-    
-    Definition term_better_ind : forall t : term, P t.
-      fix IND_PRINCIPLE 1; intros [v | f args].
-      - apply Pbase.
-      - apply Pind. induction args; constructor.
-        + apply IND_PRINCIPLE.
-        + assumption.
-    Defined.
-  End term_better_ind.
+  Set Elimination Schemes.
 
-  Section term_better_ind2.
-    Variable P : term -> Prop.
-    Hypothesis Pbase : forall v, P (TVar v).
-    Hypothesis Pind : forall (f : FuncS Σ) (args : vec term (FuncArr f)),
-        (forall st : term, V.In st args -> P st) -> P (TFunc f args).
-
-    Definition term_better_ind2 : forall t : term, P t.
-      induction t as [v | f args IH] using term_better_ind.
-      - apply Pbase.
-      - apply Pind. intros st Hin. rewrite V.Forall_forall in IH.
-        apply IH. apply Hin.
-    Defined.
-  End term_better_ind2.    
-          
+  Fixpoint term_subst (s : var -> term) (t : term) : term :=
+    match t with
+    | TVar v => s v
+    | TFunc f args => TFunc f (V.map (term_subst s) args)
+    end.
+  
   (* In term [t], substitutes all occurrences
      of the variable [x] with the term [u] *)
-  Fixpoint term_var_subst (t : term) (u : term) (x : var) : term :=
-    match t with
-    | TVar v => if v =? x then u else t
-    | TFunc f args => TFunc f (V.map (fun st => term_var_subst st u x) args)
-    end.
+  Definition term_var_subst (t : term) (x : var) (u : term) : term :=
+    term_subst (fun v => if v =? x then u else TVar v) t.
 
-  (* The set of all variables of a given term. *)
+  (* The set of all used variables of a given term. *)
   Inductive Var : term -> E.Ensemble var :=
-  | VarVar : forall (v : var), Var (TVar v) v
-  | VarFunc : forall (f : FuncS Σ) (args : vec term (FuncArr f)) (v : var),
-      V.Exists (fun t => Var t v) args -> Var (TFunc f args) v.
+  | VarVar : forall v, Var (TVar v) v
+  | VarFunc : forall f args v, V.Exists (fun t => Var t v) args -> Var (TFunc f args) v.
+
+  (* The set of all unused variables of a given term. *)
+  Inductive UnusedVar : term -> E.Ensemble var :=
+  | FV_Var : forall v w, v <> w -> UnusedVar (TVar v) w
+  | FV_Func : forall f args v, V.Forall (fun t => UnusedVar t v) args ->
+                          UnusedVar (TFunc f args) v.
 End term.
 
-Arguments TVar {Σ} _.
-Arguments TFunc {Σ} _.
-Arguments term_better_ind {Σ} _ _ _ _.
-Arguments term_var_subst {Σ} _ _ _.
-Arguments Var {Σ} _.
+Arguments term Σ : clear implicits.
 
-Declare Scope term_scope.
-Delimit Scope term_scope with term.
-Notation " t '[' x '=>' u ']' " :=
-  (term_var_subst t u x) (at level 100) : term_scope.
+Module TermNotations.
+  Declare Scope term_scope.
+  Delimit Scope term_scope with term.
+  Notation " t [ f ] " := (term_subst f t)
+                            (at level 100) : term_scope.
+  Open Scope term_scope.
+End TermNotations.
+
+Section term_ind1.
+  Context {Σ : signature} (P : term Σ -> Prop).
+  
+  Hypothesis Pbase : forall v, P (TVar v).
+  Hypothesis Pind : forall (f : FuncS Σ) args,
+      V.Forall (fun st => P st) args -> P (TFunc f args).
+  
+  Definition term_ind1 : forall t, P t.
+    fix IND_PRINCIPLE 1; intros [v | f args].
+    - apply Pbase.
+    - apply Pind. induction args; constructor.
+      + apply IND_PRINCIPLE.
+      + assumption.
+  Defined.
+End term_ind1.
+
+Require Import Coq.Program.Equality.
+
+Section term_ind2.
+  Context {Σ : signature} (P : term Σ -> Prop).
+  
+  Hypothesis Pbase : forall v, P (TVar v).
+  Hypothesis Pind : forall (f : FuncS Σ) args,
+      (forall st, V.In st args -> P st) -> P (TFunc f args).
+
+  Definition term_ind2 : forall t, P t.
+    induction t as [v | f args IH] using term_ind1.
+    - apply Pbase.
+    - apply Pind. intros st Hin. rewrite V.Forall_forall in IH.
+      apply IH. apply Hin.
+  Defined.
+End term_ind2.
 
 Section term_facts.
-  Open Scope term_scope.
-  Variable Σ : signature.
+  Import TermNotations.
+  Context {Σ : signature}.
 
-  Lemma var_not_in_Var_not_eq : forall v x, ~ E.In (@Var Σ (TVar v)) x -> v <> x.
+  Lemma var_not_in_Var_not_eq : forall v x, ~ @Var Σ (TVar v) x -> v <> x.
   Proof.
     intros v x H. intros eq. apply H. subst; constructor.
   Qed.
   
-  Lemma var_not_in_Func_not_in_args :
-    forall (f : FuncS Σ) (args : vec (term Σ) (FuncArr f)) (x : var),
-      ~ E.In (Var (TFunc f args)) x -> V.Forall (fun st => ~ E.In (Var st) x) args.
+  Lemma var_not_in_Func_not_in_args : forall (f : FuncS Σ) args x,
+      ~ Var (TFunc f args) x -> V.Forall (fun st => ~ Var st x) args.
   Proof.
     intros f args x Hnotin; rewrite V.Forall_forall; unfold E.In in *.
     intros t Hin Hvar. apply Hnotin. constructor.
@@ -86,24 +100,19 @@ Section term_facts.
     exists t; intuition.
   Qed.
     
-  Lemma term_var_subst_id : forall (t : term Σ) (x : var),
-      t [x => TVar x] = t.
+  Lemma term_subst_id : forall (t : term Σ) (x : var),
+      t [fun x => TVar x] = t.
   Proof.
-    induction t as [v | f args IH] using term_better_ind; intros x.
-    - simpl. destruct (v =? x) eqn:E.
-      + f_equal. symmetry. apply Nat.eqb_eq. apply E.
-      + reflexivity.
-    - cbn. f_equal. induction IH.
-      + reflexivity.
-      + simpl; f_equal.
-        * apply H.
-        * apply IHIH.
+    induction t as [v | f args IH] using term_ind2; intros x.
+    - reflexivity.
+    - simpl. f_equal. rewrite <- V.map_id; apply V.map_ext_in.
+      intuition.
   Qed.
     
   Lemma term_var_subst_no_occ : forall (t u : term Σ) (x : var),
-      ~ E.In (Var t) x -> t [x => u] = t.
+      ~ Var t x -> term_var_subst t x u = t.
   Proof.
-    intros t; induction t as [v | f args IH] using term_better_ind2;
+    intros t; induction t as [v | f args IH] using term_ind2;
       intros u x Hnotin; cbn.
     - destruct (v =? x) eqn:E.
       + exfalso; apply Hnotin; rewrite Nat.eqb_eq in E; subst; constructor.
@@ -114,4 +123,49 @@ Section term_facts.
       + intros Hinvar. apply Hnotin. constructor.
         apply Exists_exists. exists st; intuition.
   Qed.
+
+
+  
+  Lemma Var_not_Unused : forall (t : term Σ) v, Var t v -> ~ UnusedVar t v.
+  (* Uses axiom [Eqdep.Eq_rect_eq.eq_rect_eq] *)
+  Proof.
+    intros t v Hvar Hunused. induction t using term_ind2.
+    - inversion Hvar; inversion Hunused; intuition.
+    - dependent induction Hvar. dependent induction Hunused.
+      rewrite Exists_exists in H. rewrite V.Forall_forall in H0.
+      destruct H as [st [Hin Hvar]].
+      apply H1 with st; intuition.
+  Qed.
+
+  Lemma not_Var_Unused : forall (t : term Σ) v, ~ Var t v -> UnusedVar t v.
+  Proof.
+    intros t v Hnot; induction t using term_ind2; constructor.
+    - intros Heq; subst. apply Hnot; constructor.
+    - rewrite V.Forall_forall. intros st Hinst.
+      apply H; auto. intros Hvar. apply Hnot.
+      constructor. rewrite Exists_exists. exists st; auto.
+  Qed.
+
+  Lemma Unused_not_Var : forall (t : term Σ) v, UnusedVar t v -> ~ Var t v.
+  (* Uses axiom [Eqdep.Eq_rect_eq.eq_rect_eq] *)
+  Proof.  
+    intros t v Hunused Hvar; induction t using term_ind2.
+    - inversion Hvar; inversion Hunused; intuition.
+    - dependent destruction Hvar. rewrite Exists_exists in H. destruct H as [st [Hinst Hvarsr]].
+      apply H0 with st; auto.
+      dependent destruction Hunused.
+      rewrite V.Forall_forall in H. apply H; auto.
+  Qed.
+
+  Lemma not_Unused_Var : forall (t : term Σ) v, ~ UnusedVar t v -> Var t v.
+  Proof.
+    intros t v Hnot; induction t using term_ind2.
+    - destruct (v =? v0) eqn:E.
+      + apply Nat.eqb_eq in E; subst; constructor.
+      + apply Nat.eqb_neq in E. exfalso. apply Hnot. constructor. intuition.
+    - constructor. exfalso. apply Hnot. constructor.
+      rewrite V.Forall_forall. admit.
+  Admitted.
+  
+                                             
 End term_facts.
