Formula.v
@@ -1,29 +1,25 @@
 Require Import Base Signature Term.
 
 Section formula.
-  Variable Σ : signature.
+  Context {Σ : signature}.
 
   Inductive formula : Type :=
-  | FPred : forall R : PredS Σ, vec (term Σ) (PredArr R) -> formula
-  | FIndPred : forall R : IndPredS Σ, vec (term Σ) (IndPredArr R) -> formula
+  | FPred : forall R : PredS Σ, vec (term Σ) (pred_ar R) -> formula
+  | FIndPred : forall R : IndPredS Σ, vec (term Σ) (indpred_ar R) -> formula
   | FImp : formula -> formula -> formula
   | FNeg : formula -> formula
-  | FAll : (var -> formula) -> formula.
+  | FAll : formula -> formula.
 
   Inductive FV : formula -> E.Ensemble var :=
-  | FV_Pred :
-    forall (R : PredS Σ) (args : vec (term Σ) (PredArr R)) (v : var),
-      V.Exists (fun st => Var st v) args -> FV (FPred R args) v
-  | FV_IndPred:
-    forall (R : IndPredS Σ) (args : vec (term Σ) (IndPredArr R)) (v : var),
-      V.Exists (fun st => Var st v) args -> FV (FIndPred R args) v
-  | FV_Imp : forall (F G : formula) (v : var),
-      FV F v \/ FV G v -> FV (FImp F G) v
-  | FV_Neg : forall (F : formula) (v : var),
-      FV F v -> FV (FNeg F) v
-  | FV_All : forall (F : var -> formula) (v : var) (x : var),
-      FV (F v) x /\ x <> v -> FV (FAll F) x.
-
-  Notation " x '∈' 'FV(' F ')' " := (FV F x)
-                                      ( no associativity, at level 150).
+  | FV_Pred : forall R args v,
+      V.Forall (fun t => ~ Var t v) args -> FV (FPred R args) v
+  | FV_IndPred : forall R args v,
+      V.Forall (fun t => ~ Var t v) args -> FV (FIndPred R args) v
+  | FV_Imp_l : forall F G v, FV F v -> FV (FImp F G) v
+  | FV_Imp_r : forall F G v, FV G v -> FV (FImp F G) v
+  | FV_Neg : forall F v, FV F v -> FV (FNeg F) v
+  | FV_All : forall F v, FV F v -> FV (FAll F) (S v).
+    
 End formula.
+
+Arguments formula : clear implicits.
