Signature.v
@@ -2,13 +2,13 @@ Require Import Base.
 
 Structure signature := {
     FuncS : Type;
-    FuncArr : FuncS -> nat;
-    PredS : Type; (* ordinary predicate symbols *)
-    PredArr : PredS -> nat;
-    IndPredS : Type; (* inductive predicate symbols *)
-    IndPredArr : IndPredS -> nat
+    fun_ar : FuncS -> nat;
+    PredS : Type;
+    pred_ar : PredS -> nat;
+    IndPredS : Type;
+    indpred_ar : IndPredS -> nat
   }.
 
-Arguments FuncArr {Σ} _ : rename.
-Arguments PredArr {Σ} _ : rename.
-Arguments IndPredArr {Σ} _ : rename.
+Arguments fun_ar {Σ} f : rename.
+Arguments pred_ar {Σ} P : rename.
+Arguments indpred_ar {Σ} P : rename.
